WIP: Frame relation to freeze locals

theories/iris/logrel/relations.v
@@ -510,11 +510,11 @@ Section Relations.
     λne L oss, ([∗ list] τ; os ∈ L; oss, value_interp se τ (SAtoms os))%I.
 
   Definition frame_interp (se : semantic_env) :
-    leibnizO local_ctx -n> leibnizO wlocal_ctx -n> leibnizO instance -n> leibnizO frame -n>
+    leibnizO local_ctx -n> leibnizO wlocal_ctx -n> leibnizO frame -n>
       iPropO Σ :=
-    λne L WL inst fr,
+    λne L WL fr,
       (∃ oss_L vss_L vs_WL,
-         ⌜fr = Build_frame (concat vss_L ++ vs_WL) inst⌝ ∗
+         ⌜fr.(f_locs) = concat vss_L ++ vs_WL⌝ ∗
            ⌜result_type_interp WL vs_WL⌝ ∗
            atoms_interp (concat oss_L) (concat vss_L) ∗
            locals_interp se L oss_L)%I.
@@ -581,29 +581,39 @@ Section Relations.
     typeclasses eauto.
   Defined.
 
+  Definition mask_locs_eq (lmask : nat -> Prop) (fr fr' : frame) : Prop :=
+    forall i, lmask i -> fr.(f_locs) !! i = fr'.(f_locs) !! i.
+
+  Definition frame_rel (lmask : nat -> Prop) (fr fr' : frame) : Prop :=
+    mask_locs_eq lmask fr fr' /\ fr.(f_inst) = fr'.(f_inst).
+
   Definition label_interp
-    (se : semantic_env) (inst : instance) (WL : wlocal_ctx)
+    (se : semantic_env) (fr0 : frame) (WL : wlocal_ctx) (lmask : nat -> Prop)
     '((τs, L) : list type * local_ctx) '((n, P) : label_spec) :
     iProp Σ :=
     (match translate_types se τs with Some ts => ⌜length ts = n⌝ | None => False end ∗
        □ (∀ fr vs os θ,
+            ⌜frame_rel lmask fr0 fr⌝ -∗
+            frame_interp se L WL fr -∗
+            rt_token rti sr θ -∗
             atoms_interp os vs -∗
             values_interp se τs os -∗
-            frame_interp se L WL inst fr -∗
-            rt_token rti sr θ -∗
             P fr vs))%I.
 
-  Global Instance Persistent_label_interp se inst WL a b : Persistent (label_interp se inst WL a b).
+  Global Instance Persistent_label_interp se fr0 WL lmask a b :
+    Persistent (label_interp se fr0 WL lmask a b).
   Proof.
     destruct a, b.
     typeclasses eauto.
   Defined.
 
-  Definition labels_interp (se : semantic_env) (inst : instance) (WL : wlocal_ctx) :
+  Definition labels_interp
+    (se : semantic_env) (fr : frame) (WL : wlocal_ctx) (lmask : nat -> Prop) :
     list (list type * local_ctx) -> list label_spec -> iProp Σ :=
-    big_sepL2 (const (label_interp se inst WL)).
+    big_sepL2 (const (label_interp se fr WL lmask)).
 
-  Global Instance Persistent_labels_interp se inst WL l a : Persistent (labels_interp se inst WL l a).
+  Global Instance Persistent_labels_interp se fr WL lmask l a :
+    Persistent (labels_interp se fr WL lmask l a).
   Proof.
     apply big_sepL2_persistent'. intros; cbn.
     typeclasses eauto.
@@ -645,25 +655,27 @@ Section Relations.
 
   Definition have_instr_type_sem
     (mr : module_runtime)
-    (M : module_ctx) (F : function_ctx) (L : local_ctx) (WT : wtype_ctx) (WL : wlocal_ctx)
+    (M : module_ctx) (F : function_ctx) (L : local_ctx)
+    (WT : wtype_ctx) (WL : wlocal_ctx) (lmask : nat -> Prop)
     (es : list basic_instruction)
     '(InstrT τs1 τs2 : instruction_type) (L' : local_ctx) :
     iProp Σ :=
-    (∀ se inst fr os vs evs θ B R,
+    (∀ se fr os vs evs θ B R,
        "%Hse" ∷ ⌜sem_env_interp F se⌝ -∗
        "%Hevs" ∷ ⌜has_values evs vs⌝ -∗
-       "#Hinst" ∷ instance_interp mr M WT inst -∗
-       "#Hlabels" ∷ labels_interp se inst WL F.(fc_labels) B -∗
+       "#Hinst" ∷ instance_interp mr M WT fr.(f_inst) -∗
+       "#Hlabels" ∷ labels_interp se fr WL lmask F.(fc_labels) B -∗
        "#Hreturn" ∷ return_interp se F.(fc_return) R -∗
        "Hvs" ∷ atoms_interp os vs -∗
        "Hos" ∷ values_interp se τs1 os -∗
-       "Hframe" ∷ frame_interp se L WL inst fr -∗
+       "Hframe" ∷ frame_interp se L WL fr -∗
        "Hrt" ∷ rt_token rti sr θ -∗
        "Hfr" ∷ ↪[frame] fr -∗
        "Hrun" ∷ ↪[RUN] -∗
        CWP evs ++ es UNDER B; R
            {{ fr'; vs',
-              frame_interp se L' WL inst fr' ∗
-              ∃ os' θ, values_interp se τs2 os' ∗ atoms_interp os' vs' ∗ rt_token rti sr θ }})%I.
+              ⌜frame_rel lmask fr fr'⌝ ∗ frame_interp se L' WL fr' ∗
+                (∃ os', values_interp se τs2 os' ∗ atoms_interp os' vs') ∗
+                (∃ θ', rt_token rti sr θ') }})%I.
 
 End Relations.
