theories/iris/logrel/compat/unreachable.v
@@ -28,11 +28,12 @@ Section Fundamental.
     let fe := fe_of_context F in
     let WT := wt ++ wt' ++ wtf in
     let WL := wl ++ wl' ++ wlf in
+    let wlm := wlmask fe wl wl' in
     has_instruction_type_ok F ψ L' ->
     run_codegen (compile_instr mr fe (IUnreachable ψ)) wt wl = inr ((), wt', wl', es') ->
-    ⊢ have_instr_type_sem rti sr mr M F L WT WL es' ψ L'.
+    ⊢ have_instr_type_sem rti sr mr wlm M F L WT WL es' ψ L'.
   Proof.
-    intros fe WT WL Hok Hcg.
+    intros fe WT WL wlm Hok Hcg.
     inv_cg_emit Hcg; subst.
     destruct ψ as [τs1 τs2].
     iIntros (?????????) "@@@@@@@@@@@".
